---
output:
  html_document:
    toc: TRUE
    fig_width: 4.5
    css: /home/ebosi/github/james-chuang.github.io/_sass/_style.scss
---

```{r setup, include=FALSE}
knitr::opts_chunk$set(echo = TRUE)
```

# **CS229 Autumn 2016 Problem Set #1**

### **1. Logistic Regression**

**a.** Consider the average empirical loss (the risk) for logistic regression:
$$
\begin{align}
J(\theta) & = \frac{1}{m} \sum_{i=1}^m \log \left(1+e^{-y^{(i)}\theta^Tx^{(i)}} \right) \\
          & = - \frac{1}{m} \sum_{i=1}^m \log \left(h_\theta \left(y^{(i)} x^{(i)} \right) \right) \\
          & &h_\theta(x) & = g(\theta^Tx), \\
          & &g(z) & = \frac{1}{1+e^{-z}}
\end{align}
$$
Find the Hessian $H$ of this function, and show that for any vector $z$, it holds true that
$$
z^THz \geq 0.
$$
*Hint:* You might want to start by showing the fact that $\sum_i \sum_j z_i x_i x_j z_j = \left(x^Tz \right)^2 \geq 0$.

**Remark:** This is one of the standard ways of showing that the matrix $H$ is positive semidefinite, written "$H \succeq 0$." This implies that $J$ is convex, and has no local minima other than the global one. If you have some other way of showing $H \succeq 0$, you're also welcome to use your method instead of the one above.

$$
\begin{align}
J(\theta)                                     & = \frac{1}{m} \sum_{i=1}^m \log \left(1+e^{-y^{(i)}\theta^Tx^{(i)}} \right) \\
\frac{\partial J(\theta)}{\partial \theta_k}  & = \frac{1}{m} \sum_{i=1}^m \frac{e^{-y^{(i)}\theta^Tx^{(i)}}}{1+e^{-y^{(i)}\theta^Tx^{(i)}}} \left(-y^{(i)} x_k^{(i)} \right) \\
\frac{\partial J(\theta)}{\partial \theta_k}  & = \frac{1}{m} \sum_{i=1}^m \frac{1}{1 + e^{y^{(i)}\theta^Tx^{(i)}}} \left(-y^{(i)} x_k^{(i)} \right) \\
\frac{\partial J(\theta)}{\partial \theta_k}  & = - \frac{1}{m} \sum_{i=1}^m h_\theta \left(-y^{(i)}x^{(i)} \right) \left(y^{(i)} x_k^{(i)} \right) \\
\frac{\partial^2 J(\theta)}{\partial \theta_\ell \partial \theta_k} & = - \frac{1}{m} \sum_{i=1}^m \frac{\partial}{\partial \theta_\ell} h_\theta \left(-y^{(i)}x^{(i)} \right) \left(y^{(i)} x_k^{(i)} \right) \\
\frac{\partial^2 J(\theta)}{\partial \theta_\ell \partial \theta_k} & = - \frac{1}{m} \sum_{i=1}^m h_\theta \left(-y^{(i)} x^{(i)} \right) \left(1-h_\theta \left(-y^{(i)}x^{(i)} \right) \right) \left(-y^{(i)}x_k^{(i)} \right) \left(-y^{(i)}x_\ell^{(i)} \right) \\
& = -\frac{1}{m} \sum_{i=1}^m h_\theta \left(x^{(i)} \right) \left(1- h_\theta \left(x^{(i)} \right) \right) x_\ell^{(i)} x_k^{(i)}  ????????????????
\end{align}
$$

**b.** We have provided two data files:

  - http://cs229.stanford.edu/ps/ps1/logistic_x.txt
  - http://cs229.stanford.edu/ps/ps1/logistic_y.txt
  
These files contain the inputs $\left(x^{(i)} \in \mathbb{R}^2 \right)$ and outputs $\left(y^{(i)} \in \left\{-1,1 \right\} \right)$, respectively, for a binary classification problem, with one training example per row. Implement Newton's method for optimizing $J(\theta)$, and apply it to fit a logistic regression model to the data. Initialize Newton's method with $\theta = \vec{0}$ (the vector of all zeros). What are the coefficients $\theta$ resulting from your fit? (Remember to include the intercept term.)

```{python}
```

**c.** Plot the training data (your axes should be $x_1$ and $x_2$, corresponding to the two coordinates of the inputs, and you should use a different symbol for each point plotted to indicate whether that example has label $1$ or $-1$). Also plot on the same figure the decision boundary fit by logistic regression. (This should be a straight line showing the boundary separating the region where $h_\theta(x) > 0.5$ from where $h_\theta(x) \leq 0.5$.)

### **2. Poisson regression and the exponential family**

**a.** Consider the Poisson distribution parameterized by $\lambda$:
$$
p(y; \lambda) = \frac{e^{-\lambda}\lambda^y}{y!}
$$
Show that the Poisson distribution is in the exponential family, and clearly state what $b(y)$, $\eta$, $T(y)$, and $a(\eta)$ are.

$$
\begin{align}
p(y; \lambda) & = \frac{e^{-\lambda}\lambda^y}{y!} \\
              & = \frac{1}{y!} e^{-\lambda} e^{y \log \lambda} \\
              & = \frac{1}{y!} \exp{\left(y \log \lambda - \lambda\right)} & \text{exp. form:}\quad b(y) \exp \left(\eta^T T(y) - a(\eta) \right) \\
              \\
          b(y) & = \frac{1}{y!} \\
          T(y) & = y \\
          \eta & = \log \lambda \\
          a(\eta) & = e^\eta
\end{align}
$$
**b.** Consider performing regression using a GLM model with a Poisson response variable. What is the canonical response function for the family? (You may use the fact that a Poisson random variable with parameter $\lambda$ has mean $\lambda$.)

$$
\begin{align}
g(\eta) & = \text{E}\left[y; \eta\right] \\
        & = \lambda \\
        & = e^\eta
\end{align}
$$

**c.** For a training set $\left\{x^{(i)}, y^{(i)}; i = 1, \dots, m \right\}$, let the log-likelihood of an example be $\log p \left(y^{(i)} | x^{(i)}; \theta \right)$. By taking the derivative of the log-likelihood w.r.t. $\theta_j$, derive the stochastic gradient ascent rule for learning using a GLM model with Poisson reponses $y$ and the canonical response function.

$$
\begin{align}
p\left(y^{(i)} \mid x^{(i)}; \theta \right) & = \frac{1}{y^{(i)}!} \exp \left(\eta^T y^{(i)}-e^{\eta} \right) \\
                                            & = \frac{1}{y^{(i)}!} \exp \left(\left(\theta^Tx \right)^T y^{(i)}-e^{\theta^Tx} \right) \\
                              \ell(\theta)  & = \log \left[\frac{1}{y^{(i)}!} \exp \left({x^{(i)}}^T\theta y^{(i)}-e^{{x^{(i)}}^T\theta} \right) \right] \\
                                            & = -\log \left(y^{(i)}! \right) + {x^{(i)}}^T\theta y^{(i)}-e^{{x^{(i)}}^T\theta} \\
                \nabla_\theta \ell(\theta)  & = {x^{(i)}}^T y^{(i)} - {x^{(i)}}^Te^{{x^{(i)}}^T\theta} \\
                                            & =  \left(y^{(i)}-e^{\theta^Tx^{(i)}} \right) x_j^{(i)} \\
                                            \\
                          \therefore \frac{\partial \ell(\theta)}{\partial \theta_j} & = \left(y^{(i)}-e^{\theta^Tx^{(i)}} \right) x_j^{(i)} \\
\end{align}
$$

The stochastic gradient ascent update rule:
$$
\begin{align}
\theta & \gets \theta + \alpha \frac{\partial \ell (\theta)}{\partial \theta_j} \\
\theta & \gets \theta + \alpha \left(y^{(i)}-e^{\theta^Tx^{(i)}} \right) x_j^{(i)}
\end{align}
$$

**d.** Consider using a GLM with a reponse variable from any member of the exponential family in which $T(y) = y$, and the canonical response functino $h(x)$ for the family. Show that stochastic gradient ascent on the log-likelihood $\log p(\vec{y} |X; \theta)$ results in the update rule $\theta_i \gets \theta_i - \alpha(h(x)-y)x_i$.

### **3. Gaussian discriminant analysis**
Suppose we are given a dataset $\left\{\left(x^{(i)}, y^{(i)} \right); i = 1, \dots, m \right\}$ consisting of $m$ independent examples, where $x^{(i)} \in \mathbb{R}^n$ are $n$-dimensional vectors, and $y^{(i)} \in \{-1,1\}$. we will model the joint distribution of $(x,y)$ according to:
$$
\begin{align}
p(y) & = \begin{cases}
          \phi & \text{if } y = 1 \\
          1-\phi & \text{if } y = -1
          \end{cases} \\
p(x \mid y=-1) & = \frac{1}{(2\pi)^{\frac{n}{2}} \lvert \Sigma \rvert^{\frac{1}{2}}} \exp \left(-\frac{1}{2} \left(x-\mu_{-1} \right)^T\Sigma^{-1} \left(x-\mu_{-1} \right) \right) \\
p(x \mid y=1)  & = \frac{1}{(2\pi)^{\frac{n}{2}} \lvert \Sigma \rvert^{\frac{1}{2}}} \exp \left(-\frac{1}{2} \left(x-\mu_{1} \right)^T\Sigma^{-1} \left(x-\mu_{1} \right) \right)
\end{align}
$$
Here, the parameters of our model are $\phi$, $\Sigma$, $\mu_{-1}$, $\mu_1$. (Note that while there're two different mean vectors $\mu_{-1}$ and $\mu_1$, there's only one covariance matrix $\Sigma$.)

**a.** Suppose we have already fit $\phi$, $\Sigma$, $\mu_{-1}$, $\mu_1$, and now want to make a prediction at some new query point $x$. Show that the posterior distribution of the label at $x$ takes the form of a logistic function, and can be written
$$
p(y \mid x; \phi, \Sigma, \mu_{-1}, \mu_{1}) = \frac{1}{1+\exp \left(-y(\theta^Tx + \theta_0) \right)},
$$
where $\theta \in \mathbb{R}^n$ and the bias term $\theta_0 \in \mathbb{R}$ are some appropriate functions of $\phi$, $\Sigma$, $\mu_{-1}$, $\mu_1$. (Note: the term $\theta_0$ corresponds to introducing an extra coordinate $x_0^{(i)}=1$.)

$$
\begin{align}
p(y=1 \mid x) & = \frac{p(x \mid y=1)p(y=1)}{p(x)} \\
              & = \frac{p(x \mid y=1)p(y=1)}{p(x \mid y=1)p(y=1)+ p(x \mid y=-1)p(y=-1)} \\
              & = \frac{\frac{1}{(2\pi)^{\frac{n}{2}} \lvert \Sigma \rvert^{\frac{1}{2}}} \exp \left(-\frac{1}{2} \left(x-\mu_{1} \right)^T\Sigma^{-1} \left(x-\mu_{1} \right) \right) \left(\phi \right)  }{ \frac{1}{(2\pi)^{\frac{n}{2}} \lvert \Sigma \rvert^{\frac{1}{2}}} \exp \left(-\frac{1}{2} \left(x-\mu_{1} \right)^T\Sigma^{-1} \left(x-\mu_{1} \right) \right) \left(\phi \right) + \frac{1}{(2\pi)^{\frac{n}{2}} \lvert \Sigma \rvert^{\frac{1}{2}}} \exp \left(-\frac{1}{2} \left(x-\mu_{-1} \right)^T\Sigma^{-1} \left(x-\mu_{-1} \right) \right)\left(1-\phi \right)} \\
              & = \frac{\phi \exp \left(-\frac{1}{2} \left(x-\mu_{1} \right)^T\Sigma^{-1} \left(x-\mu_{1} \right) \right) }{\phi \exp \left(-\frac{1}{2} \left(x-\mu_{1} \right)^T\Sigma^{-1} \left(x-\mu_{1} \right) \right)  +  \left(1-\phi \right) \exp \left(-\frac{1}{2} \left(x-\mu_{-1} \right)^T\Sigma^{-1} \left(x-\mu_{-1} \right) \right)} \\
              & = \frac{1}{1+\frac{\left(1-\phi \right)\exp \left(-\frac{1}{2} \left(x-\mu_{-1} \right)^T\Sigma^{-1} \left(x-\mu_{-1} \right) \right)}{\phi \exp \left(-\frac{1}{2} \left(x-\mu_{1} \right)^T\Sigma^{-1} \left(x-\mu_{1} \right) \right)}} \\
              & = \frac{1}{1+ \exp \left(\log\left(\frac{\left(1-\phi \right)}{\phi}\right) -\frac{1}{2} \left(x-\mu_{-1} \right)^T\Sigma^{-1} \left(x-\mu_{-1} \right) + \frac{1}{2} \left(x-\mu_{1} \right)^T\Sigma^{-1} \left(x-\mu_{1} \right) \right)} \\
              & = \frac{1}{1+\exp \left(\log \left(\frac{1-\phi}{\phi}\right) -\frac{1}{2} \left(x^T \Sigma^{-1}x -2x^T \Sigma^{-1}\mu_{-1}+ \mu_{-1}^T \Sigma^{-1} \mu_{-1}\right) + \frac{1}{2} \left(x^T \Sigma^{-1}x -2x^T \Sigma^{-1}\mu_{1}+ \mu_{1}^T \Sigma^{-1} \mu_{1} \right)\right)} \\
              & = \frac{1}{1+\exp \left(\log \left(\frac{1-\phi}{\phi}\right) + x^T \Sigma^{-1} \mu_{-1} - x^T \Sigma^{-1} \mu_1 - \frac{1}{2} \mu_{-1}^T \Sigma^{-1} \mu_{-1} + \frac{1}{2} \mu_1^T\Sigma^{-1}\mu_1 \right)} \\
              & = \frac{1}{1+ \exp\left(\log\left(\frac{1-\phi}{\phi}\right) + x^T \Sigma^{-1} \left(\mu_{-1}-\mu_1 \right) - \frac{1}{2}\mu_{-1}^T\Sigma^{-1}\mu_{-1} + \mu_1^T \Sigma^{-1} \mu_1 \right)} \\
              \\
              \text{Let } \theta = \Sigma^{-1}\left(\mu_{1}-\mu_{-1} \right) &, \qquad \theta_0 = \frac{1}{2}\left(\mu_{-1}^T \Sigma^{-1} \mu_{-1}- \mu_1^T \Sigma^{-1}\mu_1 \right). \text{ Then,} \\
        p(y=1 \mid x) & = \frac{1}{1+\exp \left(-y(\theta^Tx + \theta_0) \right)}
\end{align}
$$

**b.** For this part of the problem only, you may assume $n$ (the dimension of $x$) is $1$, so that $\Sigma = [\sigma^2]$ is just a real number, and likewise the determinant of $\Sigma$ is given by $\lvert \Sigma\rvert = \sigma^2$. Given the dataset, we claim that the maximum likelihood estimates of the parameters are given by
$$
\begin{align}
\phi      & = \frac{1}{m} \sum_{i=1}^m 1 \left\{y^{(i)}=1 \right\} \\
\mu_{-1}  & = \frac{\sum_{i=1}^m 1\left\{y^{(i)}=-1 \right\}x^{(i)}}{\sum_{i=1}^m 1\left\{y^{(i)}=-1\right\}} \\
\mu_{1}   & = \frac{\sum_{i=1}^m 1\left\{y^{(i)}=1 \right\}x^{(i)}}{\sum_{i=1}^m 1\left\{y^{(i)}=1\right\}} \\
\Sigma    & = \frac{1}{m} \sum_{i=1}^m \left(x^{(i)}-\mu_{y^{(i)}} \right) \left(x^{(i)}-\mu_{y^{(i)}} \right)^T
\end{align}
$$

The log-likelihood of the data is
$$
\begin{align}
\ell \left(\phi, \mu_{-1}, \mu_1, \Sigma \right)  & = \log \prod_{i=1}^m p(x^{(i)}, y^{(i)}; \phi, \mu_{-1}, \mu_1, \Sigma) \\
                                                  & = \log \prod_{i=1}^m p(x^{(i)}\mid y^{(i)}; \phi, \mu_{-1}, \mu_1, \Sigma)p(y^{(i)};\phi).
\end{align}
$$

By maximizing $\ell$ w.r.t. the four parameters, prove that the maximum likelihood estimates of $\phi$, $\mu_{-1}$, $\mu_1$, and $\Sigma$ are indeed as given in the formulas above. (You may assume that there is at least one positive and one negative example, so that the denominators in the definition of $\mu_{-1}$ and $\mu_1$ above are non-zero.)

**c.** Without assuming that $n=1$, show that the maximum likelihood estimates of $\phi$, $\mu_{-1}$, $\mu_1$, and $\Sigma$ are as given in the formulas in part (b). [Note: If you're fairly sure that you have the answer to this part right, you don't have to do part (b), since that's just a special case.]

### **4. Linear invariance of optimization algorithms**
Consider using an iterative optimization algorithm (such as Newton's method, or gradient descent) to minimize some continuously differentiable function $f(x)$. Suppose we intialize the algorithm at $x^{(0)} = \vec{0}$. when the algorithm is run, it will produce a value of $x \in \mathbb{R}^n$ for each iteration: $x^{(1)}, x^{(2)}, \dots$.

Now, let some non-singular square matrix $A \in \mathbb{R}^{n \times n}$ be given, and define a new function $g(z) = f(Az)$. Consider using the same iterative optimization algorithm to optimize $g$ (with initialization $z^{(0)} = \vec{0}$). If the values $z^{(1)}, z^{(2)}, \dots$ produced by this method necessarily satisfy $z^{(i)} = A^{-1}x^{(i)}$ for all $i$, we say this optimization algorithm is ***invariant to linear reparameterizations***.

**a.** Show that Newton's method (applied to find the minimum of a function) is invariant to linear reparameterizations. Note that since $z^{(0)} = \vec{0} = A^{-1}x^{(0)}$, it is sufficient to show that if Newton's method applied to $f(x)$ updates $x^{(i)}$ to $x^{(i+1)}$, then Newton's method applied to $g(z)$ will update $z^{(i)} = A^{-1}x^{(i)}$ to $z^{(i+1)} = A^{-1}x^{(i+1)}$.

**b.** Is gradient descent invariant to linear reparameterizations? Justify your answer.


### **5. Regression for denoising quasar spectra**
**Introduction**. In this problem, we will apply a supervised learning technique to estimate the light spectrum of *quasars*. Quasars are luminous distant galactic nuclei that are so bright, their light overwhelms that of stars in their galaxies. Understanding properties of the spectrum of light emitted by a quasar is useful for a number of tasks: first, a number of quasar properties can be estimated from the spectra, and second, properties of the regions of the universe through which the light passes can also be evaluated (for example, we can estimate the density of neutral and ionized particles in the universe, which helps cosmologists understand the evolution and fundamental laws governing its structure). The *light spectrum* is a curve that relates the light’s intensity (formally, lumens per square meter), or luminous flux, to its wavelength. Figure 1 shows an example of a quasar light spectrum, where the wavelengths are measured in Angstroms ($\overset{\circ}{A}$), where $1 \overset{\circ}{A} = 10^{-10}$ meters.

The Lyman-$\alpha$ wavelength is a wavelength beyond which intervening particles at most negligibly interfere with light emitted from the quasar. (Interference generally occurs when a photon is absorbed by a neutral hydrogen atom, which only occurs for certain wavelengths of light.) For wavelengths greater than this Lyman-$\alpha$ wavelength, the observed light spectrum $f_{\text{obs}}$ can be modeled as a smooth spectrum $f$ plus noise:
$$
f_{\text{obs}}(\lambda) = f(\lambda) = \text{noise}(\lambda)
$$
For wavelengths below the Lyman-$\alpha$ wavelength, a region of the spectrum known as the Lyman-$\alpha$ forest, intervening matter causes attenuation of the observed signal. As light emitted by the quasar travels through regions of the universe richer in neutral hydrogen, some of it is absorbed, which we model as
$$
f_{\text{obs}}(\lambda) = \text{absorption}(\lambda) \cdot f(\lambda) + \text{noise}(\lambda)
$$
Astrophysicists and cosmologists wish to understand the absorption function, which gives information about the Lyman-$\alpha$ forest, and hence the distribution of neutral hydrogen in otherwise unreachable regions of the universe. This gives clues toward the formation and evolution of the universe. Thus, it is our goal to estimate the spectrum $f$ of an observed quasar.

**Getting the data**. We will be using data generated from the Hubble Space Telescope Faint Object Spectrograph (HST-FOS), Spectra of Active Galactic Nuclei and Quasars. We have provided two comma-separated data files located at:

  - Training set: `http://cs229.stanford.edu/ps/ps1/quasar_train.csv`
  - Test set: `http://cs229.stanford.edu/ps/ps1/quasar_test.csv`

Each file contains a single header row containing 450 numbers corresponding integral wavelengths in the interval $[1150; 1600] \overset{\circ}{A}$. The remaining lines contain relative flux measurements for each wavelength. Specifically, `quasar_train.csv` contains 200 examples and `quasar_test.csv` contains 50 examples. You may use the helper file `load_quasar_data.m` to load the data in Matlab: `http://cs229.stanford.edu/ps/ps1/load_quasar_data.m`

**a.** Locally weighted linear regression

  Consider a linear regression problem in which we want to "weight" different training examples differently. Specifically, suppose we want to minimize
  $$
  J(\theta) = \frac{1}{2} \sum_{i=1}^m w^{(i)} \left(\theta^Tx^{(i)}-y^{(i)} \right)^2
  $$
  In class, we worked out what happens for the case where all the weights $w^{(i)}$ are the same. In this problem, we will generalize some of those ideas to the weighted setting.
  
  **i.** Show that $J(\theta)$ can also be written
  $$
  J(\theta) = \left(X \theta - \vec{y} \right)^T W \left(X \theta - \vec{y} \right)
  $$
  for an appropriate diagonal matrix $W$, and where $X$ and $\vec{y}$ are as defined in class. State clearly what $W$ is.
  
  **ii.** If all the $w^{(i)}$'s equal $1$, then we saw in class that the normal equation is
  $$
  X^TX\theta = X^T \vec{y},
  $$
  and that the value of $\theta$ that minimizes $J(\theta)$ is given by $\left(X^T X \right)^{-1}X^T \vec{y}$. By finding the derivative $\nabla_\theta J(\theta)$ and setting that to zero, generalize the normal equation to this weighted setting, and give the new value of $\theta$ that minimizes $J(\theta)$ in closed form as a function of $X$, $W$, and $\vec{y}$.
  
  **iii.**
  
**b.**

  **i.**
  
  **ii.**
  
  **iii.**
  
**c.**

  **i.**
  
  **ii.**
  
  **iii.**